common/Events.v
@@ -582,7 +582,7 @@ Inductive volatile_store (ge: Senv.t):
   | volatile_store_nonvol: forall chunk m b ofs v m',
       Senv.block_is_volatile ge b = Some false ->
       Mem.store chunk m b (Ptrofs.unsigned ofs) v = Some m' ->
-      Mem.strong_non_private_stack_access m b (Ptrofs.unsigned ofs) (Ptrofs.unsigned ofs + size_chunk chunk) ->
+      strong_non_private_stack_access (Mem.stack_adt m) b (Ptrofs.unsigned ofs) (Ptrofs.unsigned ofs + size_chunk chunk) ->
       volatile_store ge chunk m b ofs v E0 m'.
 
 End WITHMEMORYMODELOPS.
@@ -765,7 +765,7 @@ Record extcall_properties (sem: extcall_sem) (sg: signature) : Prop :=
     forall ge vargs m1 t vres m2,
       sem ge vargs m1 t vres m2 ->
       Mem.unchanged_on
-        (fun b o => ~ Mem.strong_non_private_stack_access m1 b o (o+1))
+        (fun b o => ~ strong_non_private_stack_access (Mem.stack_adt m1) b o (o+1))
         m1 m2;
 
   ec_perm_frames:
@@ -1063,7 +1063,7 @@ Proof.
 - inv H. inv H0. apply Mem.unchanged_on_refl.
   eapply Mem.store_unchanged_on. eauto.
   intros. intro A; apply A. 
-  eapply Mem.strong_non_private_stack_access_inside; eauto; omega.
+  eapply strong_non_private_stack_access_inside; eauto; omega.
 - inv H.  inv H1. tauto.
   split; intros. eapply Mem.perm_store_2; eauto. eapply Mem.perm_store_1; eauto.
 - inv H. inv H2. tauto.
@@ -1160,7 +1160,7 @@ Proof.
   eapply Mem.store_unchanged_on. eauto. intros.
   intro A; apply A.
   exploit Mem.invalid_block_non_private_stack_access. eapply Mem.fresh_block_alloc; eauto.
-  unfold Mem.non_private_stack_access.
+  unfold non_private_stack_access.
   intros [[B C]|[B C]]. eapply Mem.stack_top_valid in B. eapply Mem.fresh_block_alloc in B; eauto. easy.
   eassumption.
 - inv H.  
@@ -1301,7 +1301,7 @@ Inductive extcall_memcpy_sem (sz al: Z) (ge: Senv.t):
                    \/ Ptrofs.unsigned odst + sz <= Ptrofs.unsigned osrc ->
       Mem.loadbytes m bsrc (Ptrofs.unsigned osrc) sz = Some bytes ->
       Mem.storebytes m bdst (Ptrofs.unsigned odst) bytes = Some m' ->
-      Mem.strong_non_private_stack_access m bdst (Ptrofs.unsigned odst) (Ptrofs.unsigned odst + Z.of_nat (length bytes)) ->
+      strong_non_private_stack_access (Mem.stack_adt m) bdst (Ptrofs.unsigned odst) (Ptrofs.unsigned odst + Z.of_nat (length bytes)) ->
       extcall_memcpy_sem sz al ge (Vptr bdst odst :: Vptr bsrc osrc :: nil) m E0 Vundef m'.
 
 
@@ -1355,14 +1355,14 @@ Proof.
   destruct (Mem.range_perm_storebytes m1' b2 (Ptrofs.unsigned (Ptrofs.add odst (Ptrofs.repr delta))) nil)
   as [m2' SB].
   simpl. red; intros; omegaContradiction.
-  apply Mem.lo_ge_hi_non_private_stack_access. simpl; omega.
+  apply lo_ge_hi_non_private_stack_access. simpl; omega.
   exists f, Vundef, m2'.
   split. econstructor; eauto.
   intros; omegaContradiction.
   intros; omegaContradiction.
   right; omega.
   apply Mem.loadbytes_empty. omega.
-  eapply Mem.lo_ge_hi_strong_non_private_stack_access. simpl; omega.
+  eapply lo_ge_hi_strong_non_private_stack_access. simpl; omega.
   split. constructor.
   split. eapply Mem.storebytes_empty_inject; eauto.
   split. eapply Mem.storebytes_unchanged_on; eauto. unfold loc_unmapped; intros.
@@ -1394,7 +1394,7 @@ Proof.
   eapply Mem.disjoint_or_equal_inject with (m := m1); eauto.
   apply Mem.range_perm_max with Cur; auto.
   apply Mem.range_perm_max with Cur; auto. omega.
-  eapply Mem.strong_non_private_stack_access_inside.
+  eapply strong_non_private_stack_access_inside.
   eapply Mem.strong_non_private_stack_access_inject. 4: eauto. all: eauto. rewrite LEN. rewrite nat_of_Z_eq. eauto. omega.
   omega.
   rewrite (list_forall2_length B); omega.
@@ -1421,7 +1421,7 @@ Proof.
 - intros. inv H.
   eapply Mem.storebytes_unchanged_on; eauto.
   simpl; intros. intro A; apply A.
-  eapply Mem.strong_non_private_stack_access_inside; eauto. omega. omega.
+  eapply strong_non_private_stack_access_inside; eauto. omega. omega.
 - intros. inv H.
   split; first [ now (eapply Mem.perm_storebytes_1; eauto) | now (eapply Mem.perm_storebytes_2; eauto)].
 - intros. inv H.
@@ -1710,11 +1710,10 @@ Definition external_call_stack_blocks ef := ec_stack_blocks (external_call_spec 
 Definition ec_get_frame_info (sem: extcall_sem) :=
   forall ge vargs m1 t vres m2,
     sem ge vargs m1 t vres m2 ->
-    forall b, Mem.get_frame_info m1 b = Mem.get_frame_info m2 b.
+    forall b, get_frame_info (Mem.stack_adt m1) b = get_frame_info (Mem.stack_adt m2) b.
 Lemma external_call_get_frame_info ef : ec_get_frame_info (external_call ef).
 Proof.
   red; intros.
-  unfold Mem.get_frame_info.
   erewrite external_call_stack_blocks. reflexivity. eauto.
 Qed.
 
