common/MemPerm.v
@@ -1,0 +1,54 @@
+Require Import Coqlib.
+
+(** Memory states are accessed by addresses [b, ofs]: pairs of a block
+  identifier [b] and a byte offset [ofs] within that block.
+  Each address is associated to permissions, also known as access rights.
+  The following permissions are expressible:
+- Freeable (exclusive access): all operations permitted
+- Writable: load, store and pointer comparison operations are permitted,
+  but freeing is not.
+- Readable: only load and pointer comparison operations are permitted.
+- Nonempty: valid, but only pointer comparisons are permitted.
+- Empty: not yet allocated or previously freed; no operation permitted.
+
+The first four cases are represented by the following type of permissions.
+Being empty is represented by the absence of any permission.
+*)
+
+Inductive permission: Type :=
+  | Freeable: permission
+  | Writable: permission
+  | Readable: permission
+  | Nonempty: permission.
+
+(** In the list, each permission implies the other permissions further down the
+    list.  We reflect this fact by the following order over permissions. *)
+
+Inductive perm_order: permission -> permission -> Prop :=
+  | perm_refl:  forall p, perm_order p p
+  | perm_F_any: forall p, perm_order Freeable p
+  | perm_W_R:   perm_order Writable Readable
+  | perm_any_N: forall p, perm_order p Nonempty.
+
+Hint Constructors perm_order: mem.
+
+Lemma perm_order_trans:
+  forall p1 p2 p3, perm_order p1 p2 -> perm_order p2 p3 -> perm_order p1 p3.
+Proof.
+  intros. inv H; inv H0; constructor.
+Qed.
+
+(** Each address has not one, but two permissions associated
+  with it.  The first is the current permission.  It governs whether
+  operations (load, store, free, etc) over this address succeed or
+  not.  The other is the maximal permission.  It is always at least as
+  strong as the current permission.  Once a block is allocated, the
+  maximal permission of an address within this block can only
+  decrease, as a result of [free] or [drop_perm] operations, or of
+  external calls.  In contrast, the current permission of an address
+  can be temporarily lowered by an external call, then raised again by
+  another external call. *)
+
+Inductive perm_kind: Type :=
+  | Max: perm_kind
+  | Cur: perm_kind.
