common/StackADT.v
@@ -1,0 +1,701 @@
+Require Import Coqlib.
+Require Import MemPerm.
+Require Import Memdata.
+Require Import AST.
+Require Import Values.
+Require Intv.
+
+(** This file holds definitions related to our stack abstract data type (ADT).   *)
+
+(** * Segments  *)
+
+(** Segments are building blocks of the abstract data we attach to stack blocks.
+They specify the offset at which the segment begins, and the size of the
+segment. *)
+
+Record segment :=
+  {
+    seg_ofs: Z;
+    seg_size: Z;
+  }.
+
+Definition in_segment (ofs: Z) (seg: segment) : Prop :=
+  seg_ofs seg <= ofs < seg_ofs seg + seg_size seg.
+
+Fixpoint in_segments o (l: list segment)  :=
+  match l with
+    nil => False
+  | a::r => in_segment o a \/ in_segments o r
+  end.
+
+Fixpoint segments_disjoint (l: list segment) :=
+  match l with
+    nil => True
+  | a::r => segments_disjoint r /\ forall o, in_segment o a -> ~ in_segments o r
+  end.
+
+(** * Frame information  *)
+(** A frame information [frame_info] contains a list of segments corresponding
+to the actual frame layout used at the Stacking phase, at a late compilation
+phase. This dependent record also contains well-formedness properties that
+assert the disjointness of all the segments and fix the size of the special
+segments for the return address and the link to the parent frame, which are
+known to be the size of a pointer. *)
+
+Record frame_info :=
+  {
+    frame_size: Z;
+    frame_link: segment;
+    frame_retaddr: segment;
+    frame_locals: segment;
+    frame_outgoings: segment;
+    frame_callee_saves: segment;
+    frame_data: segment;
+    frame_disjoints:
+      segments_disjoint
+        (frame_link :: frame_retaddr :: frame_locals :: frame_outgoings
+                    :: frame_callee_saves :: frame_data :: nil);
+    frame_retaddr_size:
+      seg_size frame_retaddr = size_chunk Mptr;
+    frame_link_size:
+      seg_size frame_link = size_chunk Mptr;
+  }.
+
+(** We define empty segments and frames for the sole purpose of being able to
+provide a dummy frame for initialization purposes in backend/Asmexpand.ml. These
+empty frames are never actually used in the compiler. *)
+
+Definition empty_segment : segment :=
+  {|
+    seg_ofs := 0;
+    seg_size:= 0;
+  |}.
+
+Program Definition empty_frame   : frame_info :=
+  {|
+    frame_size := 0;
+    frame_link:= {| seg_ofs := 0; seg_size := size_chunk Mptr |};
+    frame_retaddr:= {| seg_ofs := size_chunk Mptr; seg_size := size_chunk Mptr |};
+    frame_locals := empty_segment;
+    frame_outgoings := empty_segment;
+    frame_callee_saves := empty_segment;
+    frame_data := empty_segment;
+  |}.
+Next Obligation.
+  unfold in_segment; simpl.
+  intuition omega.
+Qed.
+
+(** * Frame ADT  *)
+
+(** The following definition [frame_adt] enumerates the kinds of frames that are
+relevant in CompCert. The first kind [frame_with_info] denotes a single stack
+block for each function, optionnally associated with a [frame_info]. The frame
+information will be absent in languages up to Linear, and will be the actual
+layout of the frame after that. The second kind [frame_without_info] denotes a
+set of blocks that represents the set of local variables and parameters of the
+current function. This is used in the higher-level languages from C to
+Csharpminor. *)
+
+Inductive frame_adt: Type :=
+| frame_with_info: block -> option frame_info -> frame_adt
+| frame_without_info: list block -> frame_adt.
+
+(** We model our stack of frames as a [list (option frame_adt * Z)]. The obvious
+definition would probably be [list frame_adt]. Let us explain why we differ.
+
+First, we attach a [Z] to each element of our stack to account for stack
+consumption. Each stack frame is associated with a number [n:Z] that represent
+the number of bytes that this stack frame will use once it is compiled. It is
+left as a parameter for the most part of the compiler, and we have a way to
+instantiate this parameter right at the end when we compose the simulation
+proofs of individual passes together. This number, together with properties that
+we associate with it in the memory model, are instrumental to the proof of
+correctness of merging stack blocks, in [RawAsmgen].
+
+Second, we maintain a list of [option frame_adt] instead of simply [frame_adt].
+This is again related to the way we handle the merging of stack blocks into a
+unique consecutive stack block. Indeed, once we merge different stack blocks,
+each with a different frame information representing distinct blocks, into a
+unique stack block, we cannot construct a frame ADT in the target, i.e. in the
+program with a unique stack block, that respects the frame injection that we
+define below. In short, this would break the fact that each block is mentionned
+at most once in all the frame informations of the whole stack, which is useful
+in our way of axiomatizing the memory model.
+
+Note: there would probably be a way to generalize the injection so that a block
+can be mentionned multiple times in different frame information, but preliminary
+investigations seem to indicate that this would require talking about injection
+of [frame_info] and segments, and retrieving the information attached to one
+block would require either to iterate over all the frame_adt that mention it or
+merge them all in some sense. This is still to be investigated as it would make
+the model cleaner, in my optionion. *)
+
+(** The following function [get_assoc] is used to retrieve the frame information
+attached to a given block [b]. It returns [None] when the block [b] is not part
+of the stack of frames; or when [b] is part of the stack of frames but is either
+in a list of blocks ([frame_without_info]) or in a [frame_with_info] with no
+abstract information attached. In the other case, i.e. when [b] is in a
+[frame_with_info] with some information [fi] attached, it returns [Some fi]. *)
+
+Fixpoint get_assoc (l: list (option frame_adt * Z)) (a: block) : option frame_info :=
+  match l with
+    nil => None
+  | (Some (frame_with_info b fi), n)::r => if eq_block a b then fi else get_assoc r a
+  | (Some (frame_without_info bl),n)::r => if in_dec eq_block a bl then None else get_assoc r a
+  | (None,_)::r => get_assoc r a
+  end.
+
+Definition in_frame (f: option frame_adt) (a: block) : Prop :=
+  match f with
+  | Some (frame_with_info b fi) => a = b
+  | Some (frame_without_info bl) => In a bl
+  | None => False
+  end.
+
+Lemma in_frame_dec:
+  forall f b, {in_frame f b} + {~ in_frame f b}.
+Proof.
+  destruct f; simpl; intros; auto.
+  destruct f; simpl; intros.
+  apply eq_block.
+  apply in_dec. apply eq_block.
+Defined.
+
+Fixpoint in_frames (l: list (option frame_adt * Z)) (b: block) :=
+  match l with
+    nil => False
+  | (f, _) :: r => in_frame f b \/ in_frames r b
+  end.
+
+Lemma in_frames_dec:
+  forall l b, {in_frames l b} + {~ in_frames l b}.
+Proof.
+  induction l; simpl; intros; eauto.
+  destruct a. 
+  destruct (in_frame_dec o b); auto.
+  destruct (IHl b); eauto. right; intros [A|A]; auto.
+Defined.
+
+
+Class InjectPerm :=
+  {
+    inject_perm_condition: permission -> Prop;
+    inject_perm_condition_writable: forall p, perm_order Writable p -> inject_perm_condition p;
+  }.
+
+Section INJ.
+  Context {injperm: InjectPerm}.
+
+  (** * Injection of frames *)
+
+  (** The following predicate [frame_inject' f P f1 f2] asserts that the frames
+[f1] and [f2] are in injection according to [f], a memory injection, and [P], a
+predicate that represents the permissions for the source memory [m1] in which
+[f1] lives. We identify 4 cases for frame injection. *)
+
+  Inductive frame_inject' {injperm: InjectPerm} (f: meminj) (P: block -> Z -> perm_kind -> permission -> Prop):
+    frame_adt -> frame_adt -> Prop :=
+  | frame_inject_with_info:
+      (** Identity injection for single stack block. This requires that the blocks
+        [b1] and [b2] are in injection with at most each other. In other words,
+        if [b1] is injected, then that is into [b2] at offset [0], and
+        conversely, if [b2] is the image of some block, then it is of the block
+        [b1]. *)
+      forall b1 b2 fi
+        (FB: forall b' delta, f b1 = Some (b', delta) -> b' = b2 /\ delta = 0)
+        (INJ: forall b' delta, f b' = Some (b2, delta) -> b' = b1),
+        frame_inject' f P (frame_with_info b1 fi) (frame_with_info b2 fi)
+  | frame_inject_without_info:
+      (** Identity injection for sets of blocks. We require that the sets of
+        blocks are related by injection. More precisely, if [b1] and [b2] are in
+        injection by [f], then if [b1] is in [bl1], then [b2] is in [bl2] and
+        vice-versa. *)
+      forall bl1 bl2
+        (INJlist: forall b b' delta, f b = Some (b', delta) -> (In b bl1 <-> In b' bl2)),
+        frame_inject' f P (frame_without_info bl1) (frame_without_info bl2)
+  | frame_inject_without_info_with_info:
+      (** From a set of blocks to a unique stack block. For this case, we require
+    a similar condition as in the previous case ([b ∈ bl ↔ b' = b2]). Moreover,
+    we also need to assert that if the right-hand-side has frame information
+    attached to it, then all the blocks of [bl] that inject into [b2] inject
+    into the public part of the frame information, i.e. the stack data part. *)
+      forall bl b2 ofi
+        (INDATA:
+           forall fi,
+             ofi = Some fi ->
+             forall b1 delta,
+               In b1 bl ->
+               f b1 = Some (b2, delta) ->
+               forall ofs k p,
+                 P b1 ofs k p ->
+                 inject_perm_condition p ->
+                 in_segment (ofs + delta) (frame_data fi))
+        (INJlist: forall b b' delta, f b = Some (b', delta) -> (In b bl <-> b' = b2)),
+        frame_inject' f P (frame_without_info bl) (frame_with_info b2 ofi)
+  | frame_with_info_add_info:
+      (** Going from no information to some information. Similar to the previous case. *)
+      forall b1 b2 fi
+        (INDATA: forall delta,
+            f b1 = Some (b2, delta) ->
+            forall ofs k p,
+              P b1 ofs k p ->
+              inject_perm_condition p ->
+              in_segment (ofs + delta) (frame_data fi))
+        (INJ: forall b1' b2' delta, f b1' = Some (b2', delta) -> (b1' = b1 <-> b2' = b2)),
+        frame_inject' f P (frame_with_info b1 None) (frame_with_info b2 (Some fi)).
+
+  Lemma not_in_frames_get_assoc:
+    forall l b,
+      ~ in_frames l b ->
+      get_assoc l b = None.
+  Proof.
+    induction l; simpl; intros; eauto.
+    destruct a. destruct o; auto. destruct f; auto.
+    - destruct (eq_block b b0); auto. intuition.
+    - destruct (in_dec eq_block b l0); intuition.
+  Qed.
+
+  Definition in_stack_data (lo hi: Z) (fi: frame_info) : Prop :=
+    forall ofs, lo <= ofs < hi -> in_segment ofs (frame_data fi).
+
+  Fixpoint size_stack {A} (l: list (A * Z)) : Z :=
+    match l with
+      nil => 0
+    | (a,n)::r => size_stack r + align (Z.max 0 n) 8
+    end.
+
+  Lemma frame_inject_invariant:
+    forall (P P': block -> Z -> perm_kind -> permission -> Prop) f f1 f2,
+      (forall b ofs k p b' delta, f b = Some (b', delta) -> P' b ofs k p -> P b ofs k p) ->
+      frame_inject' f P f1 f2 ->
+      frame_inject' f P' f1 f2.
+  Proof.
+    intros m m' f f1 f2 PERM FI.
+    destruct FI; try now (econstructor; eauto).
+  Qed.
+
+  Lemma list_forall2_frame_inject_invariant:
+    forall (P P': block -> Z -> perm_kind -> permission -> Prop) f f1 f2,
+      (forall b ofs k p b' delta, f b = Some (b', delta) -> P' b ofs k p -> P b ofs k p) ->
+      list_forall2 (frame_inject' f P) f1 f2 ->
+      list_forall2 (frame_inject' f P') f1 f2.
+  Proof.
+    intros m m' f f1 f2 PERM FI.
+    eapply list_forall2_imply. eauto.
+    intros.
+    eapply frame_inject_invariant; eauto.
+  Qed.
+
+  Lemma inject_frame_id m a:
+    frame_inject' inject_id m a a.
+  Proof.
+    destruct a; try (econstructor; inversion 1; tauto).
+  Qed.
+
+  Definition option_frame_inject f m1 (x y: option frame_adt * Z) :=
+    match fst x, fst y with
+      Some f1, Some f2 => frame_inject' f m1 f1 f2
+    | None, Some f => False
+    | _, _ => True
+    end /\ snd x = snd y.
+
+  Lemma list_inject_frame_id m l:
+    list_forall2 (option_frame_inject inject_id m) l l.
+  Proof.
+    induction l; simpl; intros; constructor; auto.
+    constructor; simpl; auto.
+    destruct a. simpl. destruct o; auto. eapply inject_frame_id.
+  Qed.
+
+  Lemma frame_inject_incr:
+    forall f f' m f1 f2,
+      inject_incr f f' ->
+      (forall b b' delta, f b = None -> f' b = Some (b', delta) ->
+                     ~ in_frame f1 b /\ ~ in_frame f2 b' /\
+                     forall b1 delta', in_frame f1 b1 -> f b1 = Some (b', delta') -> False)
+      ->
+      forall f1' f2',
+        f1 = Some f1' ->
+        f2 = Some f2' ->
+        frame_inject' f m f1' f2' ->
+        frame_inject' f' m f1' f2'.
+  Proof.
+    intros f f' m f1 f2 INCR NEW f1' f2' EQf1 EQf2 FI. subst.
+    inversion FI; try now (econstructor; eauto).
+    - econstructor.
+      intros.
+      destruct (f b1) as [[b delta0]|] eqn:EQ.
+      + exploit INCR. rewrite EQ. eauto. rewrite H1. inversion 1; subst.
+        eapply FB; eauto. 
+      +
+        specialize (NEW _ _ _ EQ H1).
+        destruct NEW  as (A & B & C).
+        subst. simpl in *. congruence.
+      + intros. destruct (f b') as [[b delta0]|] eqn:EQ.
+        exploit INCR. rewrite EQ. eauto. rewrite H1. inversion 1; subst.
+        eapply INJ; eauto. 
+        specialize (NEW _ _ _ EQ H1).
+        destruct NEW  as (A & B & C).
+        subst. simpl in *. congruence.
+    - econstructor; eauto. intros.
+      destruct (f b) as [[b2' delta0]|] eqn:EQ.
+      exploit INCR. rewrite EQ. eauto. rewrite H1. inversion 1; subst.
+      eapply INJlist. eauto.
+      subst. simpl in *.
+      split; intros.
+      generalize (proj1 (NEW _ _ _ EQ H1)). congruence.
+      generalize (proj1 (proj2 (NEW _ _ _ EQ H1))). congruence.
+    - econstructor; eauto. intros.
+      + destruct (f b1) as [[b' delta0]|] eqn:EQ.
+        exploit INCR. rewrite EQ. eauto. rewrite H3. inversion 1; subst.
+        eapply INDATA; eauto.
+        generalize (proj1 (NEW _ _ _ EQ H3)). subst. simpl. congruence.
+      + intros. destruct (f b) as [[b1 delta0]|] eqn:EQ.
+        exploit INCR. rewrite EQ. eauto. rewrite H1. inversion 1; subst.
+        eapply INJlist. eauto.
+        subst. simpl in *.
+        split; intros.
+        generalize (proj1 (NEW _ _ _ EQ H1)). congruence.
+        generalize (proj1 (proj2 (NEW _ _ _ EQ H1))). congruence.
+    - econstructor; eauto.
+      + intros.
+        destruct (f b1) as [[b delta']|] eqn:EQ.
+        exploit INCR. rewrite EQ. eauto. rewrite H1. inversion 1; subst.
+        eapply INDATA; eauto.
+        generalize (NEW _ _ _ EQ H1). subst; simpl. intuition congruence.
+      + intros.
+        destruct (f b1') as [[b delta']|] eqn:EQ.
+        exploit INCR. rewrite EQ. eauto. rewrite H1. inversion 1; subst.
+        eapply INJ. eauto.
+        generalize (NEW _ _ _ EQ H1). subst; simpl. intuition congruence.
+  Qed.
+
+  Lemma frame_inject_in_frame:
+    forall f m v1 v2 b b' delta,
+      frame_inject' f m v1 v2 ->
+      in_frame (Some v1) b ->
+      f b = Some (b', delta) ->
+      in_frame (Some v2) b'.
+  Proof.
+    inversion 1; intros IFF FBB; simpl in *; 
+      try first [
+            intuition congruence
+          | rewrite <- INJlist; eauto ].
+    subst. autospe. auto.
+    subst. autospe. intuition.
+  Qed.
+
+  Lemma self_inject_frame f m a:
+    (forall b, f b = None \/ f b = Some (b,0)) ->
+    frame_inject' f m a a.
+  Proof.
+    intros SELF.
+    destruct a;  constructor; auto; intros; autospe; try intuition congruence.
+    destruct (SELF b); try congruence. rewrite H in H0; inv H0. auto.
+    destruct (SELF b'); try congruence.
+    destruct (SELF b). congruence.
+    assert (b = b') by congruence. subst. tauto.
+  Qed.
+
+  Lemma self_inject_list_frames f m a:
+    (forall b, f b = None \/ f b = Some (b,0)) ->
+    list_forall2 (frame_inject' f m) a a.
+  Proof.
+    induction a; intros SELF; constructor; auto.
+    apply self_inject_frame; eauto.
+  Qed.
+
+  Lemma frame_inject_compose:
+    forall (f f' : meminj) P1 l1 l2,
+      frame_inject' f P1 l1 l2 ->
+      forall P2 l3,
+        frame_inject' f' P2 l2 l3 ->
+        (forall b1 b2 delta o k p,
+            f b1 = Some (b2, delta) ->
+            P1 b1 o k p ->
+            inject_perm_condition p ->
+            P2 b2 (o + delta) k p) ->
+        frame_inject' (compose_meminj f f') P1 l1 l3.
+  Proof.
+    intros f f' m1 l1 l2 H m2 l3 H0 PERM.
+    inv H; inv H0; unfold compose_meminj.
+    - econstructor; eauto; intros; autospe; auto.
+    - econstructor; eauto; intros; autospe; auto.
+      eapply INDATA; eauto. replace ofs with (ofs + 0). eapply PERM; eauto.
+      omega.
+      split; intros; subst; autospe; intuition subst.
+      eapply INJ; eauto.
+    - econstructor; eauto. intros; autospe. intuition.
+    - econstructor; eauto.
+      + intros; autospe.
+        replace (ofs + (z + z0)) with ((ofs + z) + z0).
+        eapply INDATA; eauto. intuition.
+        omega.
+      + intros; autospe. intuition.
+    - econstructor; eauto; intros; autospe; intuition subst.
+      rewrite Z.add_0_r. eapply INDATA; eauto.
+      eapply FB; eauto.
+      eapply H0. eapply INJ; eauto.
+    - econstructor; eauto; intros; autospe; intuition subst.
+      replace (ofs + (z + z0)) with ((ofs + z) + z0) by omega.
+      eapply INDATA0; eauto. 
+    - econstructor; eauto; intros; autospe; intuition subst.
+      rewrite Z.add_0_r. eapply INDATA; eauto.
+      eapply FB; eauto.
+      apply H0. eapply INJ0; eauto.
+  Qed.
+
+  Lemma list_frame_inject_compose:
+    forall (f f' : meminj) m1 l1 l2,
+      list_forall2 (frame_inject' f m1) l1 l2 ->
+      forall m2 l3,
+        list_forall2 (frame_inject' f' m2) l2 l3 ->
+        (forall b1 b2 delta o k p,
+            f b1 = Some (b2, delta) ->
+            m1 b1 o k p ->
+            inject_perm_condition p ->
+            m2 b2 (o + delta) k p) ->
+        list_forall2 (frame_inject' (compose_meminj f f') m1) l1 l3.
+  Proof.
+    induction 1; simpl; intros; eauto.
+    inv H. constructor.
+    inv H1.
+    constructor; auto.
+    eapply frame_inject_compose; eauto.
+    eapply IHlist_forall2; eauto.
+  Qed.
+  
+  Definition get_stack_top_blocks (l: list (option frame_adt * Z)) : list block :=
+    match l with
+      nil => nil
+    | (Some (frame_with_info b fi),_)::r => b :: nil
+    | (Some (frame_without_info bl),_)::r => bl
+    | (None,_)::r => nil
+    end.
+
+  Definition is_stack_top l (b: block) :=
+    In b (get_stack_top_blocks l).
+
+  Definition get_frame_info l : block -> option frame_info :=
+    get_assoc l.
+
+  Definition strong_non_private_stack_access l (b: block) (lo hi: Z) : Prop :=
+    match get_frame_info l b with
+      Some fi => in_stack_data lo hi fi
+    | None => True
+    end.
+
+  Definition not_retaddr_or_link_ofs l (b: block) (o: Z) : Prop :=
+    match get_frame_info l b with
+      Some fi => ~ in_segment o (frame_link fi)
+                /\ ~ in_segment o (frame_retaddr fi)
+    | None => True
+    end.
+
+  Definition range_not_retaddr_or_link_ofs l (b: block) (lo hi: Z) : Prop :=
+    forall o, lo <= o < hi -> not_retaddr_or_link_ofs l b o.
+
+  Lemma lo_ge_hi_strong_non_private_stack_access:
+    forall m b lo hi,
+      lo >= hi ->
+      strong_non_private_stack_access m b lo hi.
+  Proof.
+    red. intros.
+    destruct (get_frame_info m b); try tauto.
+    red; intros. omega.
+  Qed.
+
+  Definition non_private_stack_access m (b: block) (lo hi: Z) : Prop :=
+    (is_stack_top m b /\ range_not_retaddr_or_link_ofs m b lo hi) \/
+    (~ is_stack_top m b /\ strong_non_private_stack_access m b lo hi).
+
+  Lemma is_stack_top_dec : forall m b,
+      {is_stack_top m b} + {~is_stack_top m b}.
+  Proof.
+    intros. unfold is_stack_top. apply in_dec. 
+    apply eq_block.
+  Qed.
+
+  Lemma lo_ge_hi_non_private_stack_access:
+    forall m b lo hi,
+      lo >= hi ->
+      non_private_stack_access m b lo hi.
+  Proof.
+    unfold non_private_stack_access.
+    intros.
+    destruct (is_stack_top_dec m b);[left|right].
+    split; auto; red; intros. omega.
+    split; auto. eapply lo_ge_hi_strong_non_private_stack_access. auto.
+  Qed.
+
+  Lemma lo_ge_hi_not_retaddr:
+    forall m b lo hi,
+      lo >= hi ->
+      range_not_retaddr_or_link_ofs m b lo hi.
+  Proof.
+    unfold range_not_retaddr_or_link_ofs.
+    intros; omega. 
+  Qed.
+
+  Lemma not_in_frames_no_frame_info:
+    forall m b,
+      ~ in_frames m b ->
+      get_frame_info m b = None.
+  Proof.
+    unfold get_frame_info.
+    induction m; simpl; intros; eauto.
+    intuition.
+    destruct a, o; simpl in *. destruct f; simpl in *.
+    rewrite pred_dec_false; eauto.
+    rewrite pred_dec_false; eauto.
+    apply not_in_frames_get_assoc; auto.
+  Qed.
+
+  Lemma is_stack_top_stack_blocks:
+    forall m b,
+      is_stack_top m b <-> (exists f n r, in_frame f b /\ m = (f,n)::r).
+  Proof.
+    unfold is_stack_top, get_stack_top_blocks.
+    intros.
+    destruct m eqn:?; intuition.
+    decompose [ex and] H; intuition congruence.
+    destruct p, o. repeat eexists. destruct f; simpl in *; intuition.
+    easy.
+    destruct p,o. decompose [ex and] H; intuition. inv H2.
+    destruct f; simpl in *; intuition.
+    decompose [ex and] H. inv H2. simpl in H1. easy.
+  Qed.
+
+  Lemma in_stack_data_inside:
+    forall fi lo hi lo' hi',
+      in_stack_data lo hi fi ->
+      lo <= lo' ->
+      hi' <= hi ->
+      in_stack_data lo' hi' fi.
+  Proof.
+    intros fi lo hi lo' hi' NPSA LO HI.
+    do 2 red in NPSA |- *.
+    intros; apply NPSA. omega.
+  Qed.
+
+  Lemma strong_non_private_stack_access_inside:
+    forall m b lo hi lo' hi',
+      strong_non_private_stack_access m b lo hi ->
+      lo <= lo' ->
+      hi' <= hi ->
+      strong_non_private_stack_access m b lo' hi'.
+  Proof.
+    intros m b lo hi lo' hi' NPSA LO HI.
+    unfold strong_non_private_stack_access in *.
+    destruct (get_frame_info m b); auto.
+    eapply in_stack_data_inside in NPSA; eauto.
+  Qed.
+
+  Lemma non_private_stack_access_inside:
+    forall m b lo hi lo' hi',
+      non_private_stack_access m b lo hi ->
+      lo <= lo' ->
+      hi' <= hi ->
+      non_private_stack_access m b lo' hi'.
+  Proof.
+    intros m b lo hi lo' hi' NPSA LO HI.
+    unfold non_private_stack_access in *.
+    destruct NPSA as [[IST RNROLO]|NPSA]; auto.
+    left; split; auto.
+    red; intros. apply RNROLO. omega.
+    destruct NPSA. right. split; auto.
+    eapply strong_non_private_stack_access_inside; eauto.
+  Qed.
+
+  Lemma in_segment_dec : forall ofs seg,
+      {in_segment ofs seg} + {~in_segment ofs seg}.
+  Proof.
+    unfold in_segment. intros.
+    destruct (zle (seg_ofs seg) ofs).
+    - destruct (zlt ofs (seg_ofs seg + seg_size seg)).
+      + left. auto. 
+      + right. omega. 
+    - right. omega.
+  Qed.    
+
+  Lemma in_stack_data_dec : forall lo hi f,
+      {in_stack_data lo hi f} + {~in_stack_data lo hi f}.
+  Proof.
+    unfold in_stack_data. intros. 
+    edestruct (Intv.forall_rec (fun ofs => in_segment ofs (frame_data f))
+                               (fun ofs => ~ in_segment ofs (frame_data f))) with (lo:=lo) (hi:=hi).
+    - simpl. intros. apply in_segment_dec.
+    - auto.
+    - right. intro A.
+      destruct e as (x & IN & NIN).
+      apply NIN. apply A. auto.
+  Qed.
+
+
+  Lemma strong_non_private_stack_access_dec : forall m b lo hi,
+      {strong_non_private_stack_access m b lo hi} + 
+      {~strong_non_private_stack_access m b lo hi}.
+  Proof.
+    unfold strong_non_private_stack_access.
+    intros.
+    destruct (get_frame_info m b); auto.
+    apply in_stack_data_dec.
+  Qed.
+
+
+  Lemma not_retaddr_or_link_ofs_dec : forall m b o,
+      {not_retaddr_or_link_ofs m b o} + 
+      {~not_retaddr_or_link_ofs m b o}.
+  Proof.
+    unfold not_retaddr_or_link_ofs.
+    intros. destr.
+    destruct (in_segment_dec o (frame_link f)), (in_segment_dec o (frame_retaddr f)); intuition.  
+  Qed.
+
+  Lemma range_not_retaddr_or_link_ofs_dec : forall m b lo hi,
+      {range_not_retaddr_or_link_ofs m b lo hi} + 
+      {~range_not_retaddr_or_link_ofs m b lo hi}.
+  Proof.
+    unfold range_not_retaddr_or_link_ofs.
+    intros.
+    edestruct (Intv.forall_rec (fun ofs => lo <= ofs < hi -> not_retaddr_or_link_ofs m b ofs)
+                               (fun ofs => ~ (lo <= ofs < hi -> not_retaddr_or_link_ofs m b ofs))
+              ) with (lo0:=lo) (hi0:=hi).
+    - simpl. intros.
+      destruct (zle lo x).
+      destruct (zlt x hi).
+      destruct (not_retaddr_or_link_ofs_dec m b x); intuition.
+      left; intro; omega.
+      left; intro; omega.
+    - left; auto.
+    - right; intro O.
+      destruct e as (x & RNG & NO).
+      apply NO. intros. eauto.
+  Qed.
+
+  Lemma non_private_stack_access_dec : forall m b lo hi,
+      {non_private_stack_access m b lo hi} + 
+      {~non_private_stack_access m b lo hi}.
+  Proof.
+    intros. unfold non_private_stack_access.
+    destruct (is_stack_top_dec m b); auto.
+    destruct (range_not_retaddr_or_link_ofs_dec m b lo hi); auto.
+    destruct (strong_non_private_stack_access_dec m b lo hi); auto.
+    right; intuition.
+    right. intro A. destruct A. intuition. intuition.
+    destruct (strong_non_private_stack_access_dec m b lo hi); auto.
+    right. intuition. 
+  Qed.
+
+
+  Lemma get_frame_info_in_frames:
+    forall m b f, get_frame_info m b = Some f -> in_frames m b.
+  Proof.
+    intros.
+    destruct (in_frames_dec m b); auto.
+    rewrite not_in_frames_no_frame_info in H; auto. congruence.
+  Qed.
+
+
+End INJ.
