extraction/extraction.v
@@ -186,4 +186,4 @@ Separate Extraction
    AST.signature_main
    Floats.Float32.from_parsed Floats.Float.from_parsed
    Globalenvs.Senv.invert_symbol
-   Parser.translation_unit_file Memtype.empty_frame Coqlib.sum_left_map.
+   Parser.translation_unit_file StackADT.empty_frame Coqlib.sum_left_map.
